Graph type

CODIGO/GRAFOS/Auxiliar/Node.dfy
@@ -1,9 +1,14 @@
-class Node
+type Node = nat
+type Edge = set<Node>
+
+type Graph = (set<Node>, set<Edge>)
+
+
+function invert (graph:Graph) : (r:Graph)
 {
-  var v: string
-  var adyacentes: set<Node> 
-  constructor  (c: string) {
-    v := c;
-    adyacentes := {};  // Initialize as an empty sequence
-  }
+    var allEdges:set<Edge> := (set n1,n2 | n1 in graph.0 && n2 in graph.0 && n1 != n2 :: {n1,n2});
+    var invertGraph:Graph := (graph.0, allEdges-graph.1);
+    (invertGraph)
 }
+
+
