CODIGO/GRAFOS/Problems/CliqueProblem.dfy
@@ -1,9 +1,10 @@
 include "../Auxiliar/Node.dfy"
 
 ghost predicate Clique(graph : set<Node>, k:int)
+reads graph
 {
-  var A: set<set<Node>> := (set node | node in graph :: {node});
-  exists s:set<Node> :: isClique(s,A) && |s| <= k && s <= graph
+  var A: set<set<Node>> := (set node, adj | node in graph && adj in node.adyacentes:: {node, adj});
+  exists s:set<Node> :: isClique(s,A) && |s| >= k && s <= graph
 }
 
 ghost predicate isClique(s:set<Node>, A:set<set<Node>>)
