CODIGO/GRAFOS/Problems/IndependentSet.dfy
@@ -1,8 +1,9 @@
 include "../Auxiliar/Node.dfy"
 
 ghost predicate IndependentSet(graph:set<Node>, k:int)
+reads graph
 {
-  var A: set<set<Node>> := (set node | node in graph :: {node, node.adyacentes} /*adyacent*/);
+  var A: set<set<Node>> := (set node, adj | node in graph && adj in node.adyacentes:: {node, adj});
   exists s:set<Node> :: isIndependentSet(s,A) && |s| >= k && s <= graph
 }
 
@@ -10,4 +11,3 @@ ghost predicate isIndependentSet(s:set<Node>, A:set<set<Node>>)
 {
   forall a | a in A :: |s * a| <= 1
 }
-
